examples/typecheck_examples.sh
@@ -21,7 +21,7 @@ function typecheck {
   fi
   if [ "$3" == "fst" ];
   then
-    echo "    extracting F* to $fstar_file..."
+    echo "    extracting F* ..."
     cargo hacspec -o $fstar_file $1
   fi
   if [ "$4" == "json" ];
@@ -37,15 +37,15 @@ cargo clean
 cargo build
 cargo install --path language
 typecheck hacspec-chacha20             ec      fst    json  Hacspec.Chacha20.fst
-typecheck hacspec-chacha20poly1305     ec      fst    json
-typecheck hacspec-poly1305             ec      fst    json
+typecheck hacspec-chacha20poly1305     ec      fst    json  Hacspec.Chacha20Poly1305.fst
+typecheck hacspec-poly1305             ec      fst    json  Hacspec.Poly1305.fst
 typecheck hacspec-curve25519           ec      fst    json
 typecheck hacspec-hkdf                 ec      fst    json
 typecheck hacspec-hmac              no-ec      fst    json
 typecheck hacspec-sha256            no-ec      fst    json
 typecheck hacspec-ntru-prime           ec      fst    json
 typecheck hacspec-p256                 ec      fst    json
-typecheck hacspec-riot-bootloader      ec      fst    json
+typecheck hacspec-riot-bootloader      ec      fst    json  Hacspec.Riot.fst
 typecheck hacspec-sha3              no-ec      fst    json
 typecheck hacspec-gimli                ec      fst    json
 typecheck hacspec-bls12-381         no-ec   no-fst    json
